Update event-handler file to operate on entries rather than IO actions to be compatible with generic reduction proof approach

ironfleet/src/Dafny/Distributed/Concur/EventHandler.i.dfy
@@ -5,125 +5,96 @@ module EventHandlerModule {
     import opened DistributedSystemModule
     import opened ReductionModule
 
-    predicate IOActionsCompatibleWithReductionUsingPivot(ios:seq<IOAction>, pivot:int)
+    function CombineIOLevelEntriesIntoIOs(entries:seq<Entry>) : seq<IOAction>
     {
-           0 <= pivot < |ios|
-        && (forall i :: 0 <= i < pivot ==> IOActionIsRightMover(ios[i]))
-        && (forall i :: pivot < i < |ios| ==> IOActionIsLeftMover(ios[i]))
-    }
-
-    predicate IOActionsCompatibleWithReduction(ios:seq<IOAction>)
-    {
-        |ios| == 0 || exists pivot :: IOActionsCompatibleWithReductionUsingPivot(ios, pivot)
-    }
-
-    lemma lemma_IfIOActionsCompatibleWithReductionAndOneIsntRightMoverThenRestAreLeftMovers(ios:seq<IOAction>, i:int, j:int)
-        requires 0 <= i < j < |ios|;
-        requires IOActionsCompatibleWithReduction(ios);
-        requires !IOActionIsRightMover(ios[i]);
-        ensures  IOActionIsLeftMover(ios[j]);
-        decreases j;
-    {
-        var pivot :| IOActionsCompatibleWithReductionUsingPivot(ios, pivot);
-        assert !(i < pivot);
-        assert j > pivot;
-    }
-
-    lemma lemma_IfIOActionsCompatibleWithReductionThenSuffixIs(ios:seq<IOAction>)
-        requires |ios| > 0;
-        requires IOActionsCompatibleWithReduction(ios);
-        ensures  IOActionsCompatibleWithReduction(ios[1..]);
-    {
-        var ios' := ios[1..];
-        if |ios'| == 0 {
-            return;
-        }
-        
-        var pivot :| IOActionsCompatibleWithReductionUsingPivot(ios, pivot);
-        if pivot == 0 {
-            assert IOActionsCompatibleWithReductionUsingPivot(ios', 0);
-        }
-        else {
-            assert IOActionsCompatibleWithReductionUsingPivot(ios', pivot-1);
-        }
-    }
-
-    function CombineIOActions(ios:seq<IOAction>) : seq<IOAction>
-    {
-        if |ios| == 0 then
+        if |entries| == 0 then
             []
         else
-            var head_action := ios[0];
-            if head_action.IOActionUpdateLocalState? || head_action.IOActionStutter? then
-                CombineIOActions(ios[1..])
+            var head_entry := entries[0];
+            if !head_entry.EntryAction? || !head_entry.action.ActionIO? then
+                CombineIOLevelEntriesIntoIOs(entries[1..])
             else
-                [head_action] + CombineIOActions(ios[1..])
+                var head_io := head_entry.action.io;
+                if head_io.IOActionUpdateLocalState? || head_io.IOActionStutter? then
+                    CombineIOLevelEntriesIntoIOs(entries[1..])
+                else
+                    [head_io] + CombineIOLevelEntriesIntoIOs(entries[1..])
     }
 
-    function CombineIOActionsIntoDSActionHostEventHandler(ios:seq<IOAction>) : DSAction
-        ensures CombineIOActionsIntoDSActionHostEventHandler(ios).DSActionHostEventHandler?;
+    function CombineIOLevelEntriesIntoDSEntry(actor:Actor, entries:seq<Entry>) : Entry
+        ensures var result := CombineIOLevelEntriesIntoDSEntry(actor, entries);
+                result.EntryAction? && result.actor == actor && result.action.ActionDS? && result.action.ds.DSActionHostEventHandler?;
     {
-        DSActionHostEventHandler(CombineIOActions(ios))
+        EntryAction(actor, ActionDS(DSActionHostEventHandler(CombineIOLevelEntriesIntoIOs(entries))))
     }
 
-    lemma lemma_CombineIOActionsPreservesNonUpdateStutters(ios:seq<IOAction>, io:IOAction)
-        requires io in ios;
-        requires !io.IOActionUpdateLocalState?;
-        requires !io.IOActionStutter?;
-        ensures  io in CombineIOActions(ios);
+    lemma lemma_CombineIOLevelEntriesIntoIOsIntroducesNoNewIOs(entries:seq<Entry>, io:IOAction) returns (entry:Entry)
+        requires io in CombineIOLevelEntriesIntoIOs(entries);
+        ensures  entry in entries;
+        ensures  entry.EntryAction?;
+        ensures  entry.action.ActionIO?;
+        ensures  entry.action.io == io;
     {
-    }
+        assert |entries| > 0;
 
-    lemma lemma_CombineIOActionsIntroducesNoNewIOs(ios:seq<IOAction>, io:IOAction)
-        requires io in CombineIOActions(ios);
-        ensures  io in ios;
-    {
-    }
-
-    lemma lemma_EffectOfCombiningIOActionsMatchesEffectOfDoingIOActions(
-        actor:Actor,
-        io_actions:seq<IOAction>,
-        ds_action:DSAction,
-        states:seq<DistributedSystemState>
-        )
-        requires actor.HostActor?;
-        requires |states| == |io_actions| + 1;
-        requires forall i :: 0 <= i < |io_actions| ==> DistributedSystemNextIOAction(states[i], states[i+1], actor, io_actions[i]);
-        requires ds_action == CombineIOActionsIntoDSActionHostEventHandler(io_actions);
-        requires IOActionsCompatibleWithReduction(io_actions);
-        ensures  DistributedSystemNextDSAction(states[0], states[|io_actions|], actor, ds_action);
-    {
-        if |io_actions| == 0 {
+        var head_entry := entries[0];
+        if !head_entry.EntryAction? || !head_entry.action.ActionIO? {
+            entry := lemma_CombineIOLevelEntriesIntoIOsIntroducesNoNewIOs(entries[1..], io);
             return;
         }
 
-        var ds_action_all_but_last := CombineIOActionsIntoDSActionHostEventHandler(io_actions[1..]);
-        lemma_IfIOActionsCompatibleWithReductionThenSuffixIs(io_actions);
-        lemma_EffectOfCombiningIOActionsMatchesEffectOfDoingIOActions(actor, io_actions[1..], ds_action_all_but_last, states[1..]);
+        var head_io := head_entry.action.io;
+        if head_io.IOActionUpdateLocalState? || head_io.IOActionStutter? {
+            entry := lemma_CombineIOLevelEntriesIntoIOsIntroducesNoNewIOs(entries[1..], io);
+            return;
+        }
 
-        var ds := states[0];
-        var ds' := states[|io_actions|];
-        var ios := ds_action.ios;
+        if head_io == io {
+            entry := head_entry;
+            return;
+        }
 
-        var first_action := io_actions[0];
+        entry := lemma_CombineIOLevelEntriesIntoIOsIntroducesNoNewIOs(entries[1..], io);
+    }
 
-        if first_action.IOActionSend? {
-            forall io | io in io_actions
-                ensures !io.IOActionReceive?
-            {
-                var i :| 0 <= i < |io_actions| && io_actions[i] == io;
-                if i != 0 {
-                    lemma_IfIOActionsCompatibleWithReductionAndOneIsntRightMoverThenRestAreLeftMovers(io_actions, 0, i);
-                }
-            }
-    
+    lemma lemma_EffectOfCombiningIOLevelEntriesMatchesEffectOfDoingIOLevelEntries(
+        actor:Actor,
+        entries:seq<Entry>,
+        entry:Entry,
+        db:seq<DistributedSystemState>
+        )
+        requires actor.HostActor?;
+        requires |db| == |entries| + 1;
+        requires forall i :: 0 <= i < |entries| ==> DistributedSystemNextEntryAction(db[i], db[i+1], entries[i]);
+        requires forall i :: 0 <= i < |entries| ==> GetEntryActor(entries[i]) == actor && GetEntryLevel(entries[i]) == const_IOLevel();
+        requires entry == CombineIOLevelEntriesIntoDSEntry(actor, entries);
+        requires EntriesCompatibleWithReduction(entries);
+        ensures  DistributedSystemNextEntryAction(db[0], db[|entries|], entry);
+    {
+        if |entries| == 0 {
+            return;
+        }
+
+        var entry_all_but_last := CombineIOLevelEntriesIntoDSEntry(actor, entries[1..]);
+        lemma_IfEntriesCompatibleWithReductionThenSuffixIs(entries);
+        lemma_EffectOfCombiningIOLevelEntriesMatchesEffectOfDoingIOLevelEntries(actor, entries[1..], entry_all_but_last, db[1..]);
+
+        var ds := db[0];
+        var ds' := db[|entries|];
+        var ios := entry.action.ds.ios;
+
+        var first_entry := entries[0];
+
+        if first_entry.EntryAction? && first_entry.action.ActionIO? && first_entry.action.io.IOActionSend? {
             forall io | io in ios && io.IOActionReceive?
                 ensures false;
             {
-                lemma_CombineIOActionsIntroducesNoNewIOs(io_actions, io);
+                var found_entry := lemma_CombineIOLevelEntriesIntoIOsIntroducesNoNewIOs(entries, io);
+                var i :| 0 <= i < |entries| && entries[i] == found_entry;
+                lemma_IfEntriesCompatibleWithReductionAndOneIsntRightMoverThenRestAreLeftMovers(entries, 0, i);
             }
         }
-
     }
+
 
 }
